Refactor and additions to epoch example

src/examples/epoch_persistency.v
@@ -1,6 +1,6 @@
 From stdpp Require Import numbers countable.
 
-From iris.algebra Require Import excl agree csum.
+From iris.algebra Require Import excl agree csum gset.
 From iris.proofmode Require Import tactics.
 
 From self.base Require Import primitive_laws.
@@ -9,10 +9,10 @@ From self.high Require Import dprop.
 
 From self.lang Require Import notation lang.
 From self.algebra Require Import view.
-From self.base Require Import primitive_laws class_instances.
+From self.base Require Import primitive_laws class_instances crash_borrow.
 From self.high Require Import proofmode wpc_proofmode.
 From self.high Require Import dprop resources crash_weakestpre weakestpre
-     weakestpre_na recovery_weakestpre lifted_modalities modalities
+     weakestpre_na weakestpre_at recovery_weakestpre lifted_modalities modalities crash_borrow
      post_crash_modality protocol no_buffer abstract_state_instances locations protocol.
 From self.high.modalities Require Import fence.
 
@@ -41,10 +41,12 @@ Section program.
 
 End program.
 
+Definition x_state := option (bool + bool).
+
 (* One shot resource algebra that we use in this example. *)
-Definition one_shotR := csumR (exclR unitO) (agreeR ZO).
+Definition one_shotR := csumR (exclR unitO) (agreeR (leibnizO x_state)).
 Definition Pending : one_shotR := Cinl (Excl ()).
-Definition Shot (n : Z) : one_shotR := Cinr (to_agree n).
+Definition Shot (n : x_state) : one_shotR := Cinr (to_agree n).
 
 Class one_shotG Σ := { one_shot_inG :> inG Σ one_shotR }.
 Definition one_shotΣ : gFunctors := #[GFunctor one_shotR].
@@ -52,24 +54,60 @@ Global Instance subG_one_shotΣ {Σ} : subG one_shotΣ Σ → one_shotG Σ.
 Proof. solve_inG. Qed.
 
 Section proof.
-  Context `{nvmFixedG Σ, nvmDeltaG Σ, one_shotG Σ }.
+  Context `{nvmFixedG Σ, nvmDeltaG Σ, one_shotG Σ, inG Σ (gset_disjR nat) }.
 
-  Context (x y z : loc).
+  Context (x y z : loc) (γag : gname) (γtok : gname).
 
   (* Protocol for [x]. *)
 
-  Program Definition prot_x :=
-    {| pred (n : Z) (v : val) _ := ⌜ v = #x ⌝%I;
-      bumper b := b; |}.
-  Next Obligation. iIntros (???) "H". iCrashFlush. done. Qed.
+  Definition zero : x_state := None.
+  Definition one_l : x_state := Some (inl false).
+  Definition one_r : x_state := Some (inr false).
+  Definition two_l : x_state := Some (inl true).
+  Definition two_r : x_state := Some (inr true).
+
+  Definition x_state_to_nat (s : x_state) : nat :=
+    match s with
+      None => 0
+    | Some (inl false) => 1
+    | Some (inr false) => 1
+    | Some (inl true) => 2
+    | Some (inr true) => 2
+    end%I.
+
+  Definition tok0 : dProp Σ := ⎡ own γtok (GSet {[ 0 ]}) ⎤.
+  Definition tok1 : dProp Σ := ⎡ own γtok (GSet {[ 1 ]}) ⎤.
+  Definition tok2 : dProp Σ := ⎡ own γtok (GSet {[ 2 ]}) ⎤.
+  Definition tokFin1 : dProp Σ := ⎡ own γtok (GSet {[ 3 ]}) ⎤.
+  Definition tokFin2 : dProp Σ := ⎡ own γtok (GSet {[ 4 ]}) ⎤.
+
+  Program Definition prot_x := {|
+    pred s v _ := (
+      ⌜ v = #(x_state_to_nat s) ⌝ ∗
+      (* (⌜ s = zero ⌝ ∨ *)
+      (*   ⌜ s = two_l ⌝ ∗ tok2 ∗ (tokFin1 ∨ tokFin2) ∨ *)
+      (*   ⌜ s = one_l ⌝ ∗ tok1 ∗ tokFin1 ∨ *)
+      (*   ⌜ s = one_r ⌝ ∗ tok1 ∗ (tokFin1 ∨ tokFin2) ∨ *)
+      (*   ⌜ s = two_r ⌝ ∗ tok2 ∗ tokFin2))%I *)
+      match s with
+        None => tok0
+      | Some (inl true) => tok2 ∗ (tokFin1 ∨ tokFin2)
+      | Some (inl false) => tok1 ∗ tokFin1
+      | Some (inr false) => tok1 ∗ (tokFin1 ∨ tokFin2)
+      | Some (inr true) => tok2 ∗ tokFin2
+      end)%I
+    ;
+    bumper b := b;
+  |}.
+  Next Obligation. iIntros (? [[[|]|[|]]|] ?) "H"; simpl; iCrashFlush; done. Qed.
 
   (* Protocol for [y]. *)
 
-  Program Definition prot_y (γ : gname) :=
+  Program Definition prot_y :=
     {| pred (b : bool) (v : val) _ :=
         match b with
           false => ⌜ v = #0 ⌝
-        | true => ⌜ v = #1 ⌝ ∗ ⎡ own γ (Shot 2) ⎤
+        | true => ⌜ v = #1 ⌝ ∗ ⎡ own γag (Shot two_r) ⎤
         end%I;
       bumper b := b; |}.
   Next Obligation. Admitted.
@@ -77,14 +115,103 @@ Section proof.
 
   (* Protocol for [z]. *)
 
-  Program Definition prot_z (γ : gname) :=
+  Program Definition prot_z :=
     {| pred (b : bool) (v : val) _ :=
         match b with
           false => ⌜ v = #0 ⌝
-        | true => ⌜ v = #1 ⌝ ∗ ∃ n, ⎡ own γ (Shot n) ⎤ ∗ flush_lb x prot_x n
+        | true => ⌜ v = #1 ⌝ ∗ ∃ n, ⎡ own γag (Shot n) ⎤ ∗ flush_lb x prot_x n
         end%I;
       bumper b := b; |}.
   Next Obligation. Admitted.
   Next Obligation. Admitted.
+  Next Obligation. Admitted.
+
+  Definition crash_condition {hD : nvmDeltaG Σ} : dProp Σ :=
+    ∃ (yb bz : bool),
+      ⎡ is_at_loc x ⎤ ∗
+      persist_lb x prot_x None ∗
+      (* y *)
+      persist_lb y prot_y false ∗
+      y ↦_{prot_y} [yb] ∗
+      (* z *)
+      persist_lb z prot_z false ∗
+      z ↦_{prot_z} [bz].
+
+  Definition left_crash_condition {hD : nvmDeltaG Σ} : dProp Σ :=
+    ⎡ is_at_loc x ⎤ ∗ persist_lb x prot_x None.
+
+ (*  Lemma left_prog_spec : *)
+ (*    tok2 -∗ tokFin1 -∗ ⎡ is_at_loc x ⎤ -∗ persist_lb x prot_x None -∗ *)
+ (*    WPC leftProg x @ ⊤ *)
+ (*      {{ v, store_lb x prot_x two_l ∨ store_lb x prot_x two_r }} *)
+ (*      {{ <PC> _, True }}. *)
+ (*  Proof. *)
+ (*    iIntros "tok tokFin #atLoc #perLb". *)
+ (*    rewrite /leftProg. *)
+ (*    iApply wpc_atomic_no_mask. *)
+ (*    iSplit. { iCrash. done. } *)
+ (*    iApply ( *)
+ (*        wp_store_at_strong _ (λ s, ⌜ s = two_l ∨ s = two_r ⌝)%I with "[$atLoc tok tokFin]"). *)
+ (*    { iDestruct (persist_lb_to_store_lb with "perLb") as "$". *)
+ (*      iIntros (s_l v_l le). *)
+ (*      (* [s_l] can either be [zero] or [one_r]. *) *)
+ (*      destruct (decide (s_l = zero)) as [->|neq]. *)
+ (*      - iExists two_l. *)
+ (*        iSplit. { *)
+ (*          iIntros (? [[[|]|[|]]|] ??) "H1 [-> H2]"; simpl. *)
+ (*          * admit. *)
+ (*          * admit. *)
+ (*          * admit. *)
+ (*          * admit. *)
+ (*          * admit. } *)
+ (* (* simplify_eq. *) *)
+ (*          (* iSplit; first done. *) *)
+ (*          (* admit. } *) *)
+ (*        iSplitL "". { iModIntro. iIntros "$". rewrite left_id. iAccu. } *)
+ (*        iIntros "_". *)
+ (*        iSplit; last (iLeft; done). *)
+ (*        iSplitPure; first done. *)
+ (*        iRight. iLeft. iFrame. done. *)
+ (*      - iExists two_r. *)
+ (*        iSplitL "". { admit. } *)
+ (*        simpl. iSplitPure; first done. *)
+ (*        iRight. iRight. iRight. iRight. iFrame. done. *)
+ (*      } *)
+ (*  Qed. *)
+
+  Lemma right_prog_spec :
+    tokFin1 -∗ tok2 -∗
+    ⎡ pre_borrow ⎤ -∗
+    (* x *)
+    ⎡ is_at_loc x ⎤ -∗
+    persist_lb x prot_x None -∗
+    (* y *)
+    persist_lb y prot_y false -∗
+    y ↦_{prot_y} [false] -∗
+    (* z *)
+    persist_lb z prot_z false -∗
+    z ↦_{prot_z} [false] -∗
+    WPC prog x y z @ ⊤
+      {{ v, True }}
+      {{ <PC> _, crash_condition }}.
+  Proof. Admitted.
+
+  Lemma prog_spec :
+    tok1 -∗ tok2 -∗
+    tokFin1 -∗ tokFin2 -∗
+    ⎡ pre_borrow ⎤ -∗
+    (* x *)
+    ⎡ is_at_loc x ⎤ -∗
+    persist_lb x prot_x None -∗
+    (* y *)
+    persist_lb y prot_y false -∗
+    y ↦_{prot_y} [false] -∗
+    (* z *)
+    persist_lb z prot_z false -∗
+    z ↦_{prot_z} [false] -∗
+    WPC prog x y z @ ⊤
+      {{ v, True }}
+      {{ <PC> _, crash_condition }}.
+  Proof. Admitted.
 
 End proof.
