src/examples/flush_fence.v
@@ -1,0 +1,231 @@
+From iris.proofmode Require Import tactics.
+
+From self.base Require Import primitive_laws.
+From self.lang Require Import lang.
+From self.high Require Import dprop.
+
+From self.lang Require Import notation lang.
+From self.algebra Require Import view.
+From self.base Require Import primitive_laws class_instances.
+From self.high Require Import proofmode wpc_proofmode.
+From self.high Require Import dprop resources crash_weakestpre weakestpre
+     weakestpre_na recovery_weakestpre lifted_modalities modalities
+     post_crash_modality protocol no_buffer abstract_state_instances locations protocol.
+From self.high.modalities Require Import fence.
+
+Section program.
+
+  Definition incr_both (ℓa ℓb : loc) : expr :=
+    #ℓa <-_NA #1 ;;
+    Flush #ℓa ;;
+    Fence ;;
+    #ℓb <-_NA #1.
+
+  Definition recover (ℓa ℓb : loc) : expr :=
+    let: "a" := !_NA #ℓa in
+    let: "b" := !_NA #ℓb in
+    if: "a" < "b"
+    then #() #() (* Get stuck. *)
+    else #().
+
+End program.
+
+(* This is a simple example with a flush and a fence. *)
+Section specification.
+  Context `{nvmFixedG Σ, nvmDeltaG Σ}.
+
+  (* After a crash the following is possible: [a = 0, b = 0], [a = 1, b = 0],
+  and [a = 1, b = 1]. The case that is _not_ possible is: [a = 0, b = 1]. *)
+
+  (* Predicate used for the location [a]. *)
+  Program Definition ϕa : LocationProtocol nat :=
+    {| pred := λ n v _, ⌜v = #n⌝%I;
+       bumper n := n |}.
+  Next Obligation. iIntros. by iApply post_crash_flush_pure. Qed.
+
+  (* Predicate used for the location [b]. *)
+  Program Definition ϕb ℓa : LocationProtocol nat :=
+    {| pred := λ n v _, (⌜v = #n⌝ ∗ ∃ m, ⌜ n ≤ m ⌝ ∗ flush_lb ℓa ϕa m)%I;
+       bumper n := n |}.
+  Next Obligation.
+    iIntros (????) "[% lb]".
+    iDestruct "lb" as (m ?) "lb".
+    iCrashFlush.
+    iDestruct "lb" as (??) "(? & H)".
+    iPureGoal; first done.
+    iExists _.
+    iDestruct (persist_lb_to_flush_lb with "H") as "$".
+    iPureIntro. etrans; done.
+  Qed.
+
+  Definition crash_condition {hD : nvmDeltaG Σ} ℓa ℓb : dProp Σ :=
+    ("pts" ∷ ∃ (na nb : nat),
+     "aPer" ∷ persist_lb ℓa ϕa na ∗
+     "bPer" ∷ persist_lb ℓb (ϕb ℓa) nb ∗
+     "aPts" ∷ ℓa ↦_{ϕa} [na] ∗
+     "bPts" ∷ ℓb ↦_{ϕb ℓa} [nb])%I.
+
+  Lemma prove_crash_condition {hD : nvmDeltaG Σ} ℓa ℓb na nb (ssA ssB : list nat) :
+    persist_lb ℓa ϕa na -∗
+    persist_lb ℓb (ϕb ℓa) nb -∗
+    ℓa ↦_{ϕa} ssA -∗
+    ℓb ↦_{ϕb ℓa} ssB -∗
+    <PC> hG, crash_condition ℓa ℓb.
+  Proof.
+    iIntros "perA perB aPts bPts".
+    iCrash.
+    iDestruct "perA" as (na' ?) "[perA #recA]".
+    iDestruct "perB" as (nb' ?) "[perB #recB]".
+    iDestruct (crashed_in_if_rec with "recA aPts") as (??) "[ptsA recA']".
+    iDestruct (crashed_in_agree with "recA recA'") as %<-.
+    iDestruct (crashed_in_if_rec with "recB bPts") as (??) "[ptsB recB']".
+    iDestruct (crashed_in_agree with "recB recB'") as %<-.
+    iExists na', nb'.
+    iFrame.
+  Qed.
+
+  Lemma wp_incr_both ℓa ℓb s E :
+    ⊢ persist_lb ℓa ϕa 0 -∗
+      persist_lb ℓb (ϕb ℓa) 0 -∗
+      ℓa ↦_{ϕa} [0] -∗
+      ℓb ↦_{ϕb ℓa} [0] -∗
+      WPC (incr_both ℓa ℓb) @ s; E
+        {{ λ _, ℓa ↦_{ϕa} [0; 1] ∗ ℓb ↦_{ϕb ℓa} [0; 1] }}
+        {{ <PC> _, crash_condition ℓa ℓb }}.
+  Proof.
+    iIntros "#aPer #bPer aPts bPts".
+    rewrite /incr_both.
+
+    (* The first store *)
+    wpc_bind (_ <-_NA _)%E.
+    iApply wpc_atomic_no_mask.
+    iSplit. { iApply (prove_crash_condition with "aPer bPer aPts bPts"). }
+    iApply (@wp_store_na with "[$aPts]").
+    { reflexivity. }
+    { suff leq : (0 ≤ 1); first apply leq. lia. }
+    { done. }
+    simpl.
+    iNext. iIntros "aPts".
+    iSplit. { iModIntro. iApply (prove_crash_condition with "aPer bPer aPts bPts"). }
+    iModIntro.
+    wpc_pures.
+    { iApply (prove_crash_condition with "aPer bPer aPts bPts"). }
+
+    (* The write back *)
+    wpc_bind (Flush _)%E.
+    iApply wpc_atomic_no_mask.
+    iSplit. { iApply (prove_crash_condition with "aPer bPer aPts bPts"). }
+    iApply (wp_flush_ex with "aPts"); first reflexivity.
+    iNext.
+    iIntros "(aPts & #pLowerBound & _)".
+    iSplit; first iApply (prove_crash_condition with "aPer bPer aPts bPts").
+    iModIntro.
+    wpc_pures.
+    { iApply (prove_crash_condition with "aPer bPer aPts bPts"). }
+
+    (* The fence. *)
+    wpc_bind (Fence)%E.
+    iApply wpc_atomic_no_mask.
+    iSplit; first iApply (prove_crash_condition with "aPer bPer aPts bPts").
+    iApply wp_fence. iModIntro. iModIntro.
+    iSplit. {
+      iModIntro. iApply (prove_crash_condition with "aPer bPer aPts bPts"). }
+    iModIntro.
+    wpc_pures. { iApply (prove_crash_condition with "aPer bPer aPts bPts"). }
+
+    (* The last store *)
+    iApply wpc_atomic_no_mask.
+    iSplit. { iApply (prove_crash_condition with "aPer bPer aPts bPts"). }
+    iApply (wp_store_na with "[$bPts]").
+    { reflexivity. }
+    { suff leq : (0 ≤ 1); first apply leq. lia. }
+    { iFrame "#". iPureGoal; first done. naive_solver. }
+    iNext. iIntros "bPts".
+    iSplit.
+    { iModIntro. iApply (prove_crash_condition with "aPer bPer aPts bPts"). }
+    iModIntro.
+    iFrame "aPts bPts".
+  Qed.
+
+  Lemma wpc_recover `{hD : nvmDeltaG Σ} ℓa ℓb s E :
+    crash_condition ℓa ℓb -∗
+    WPC recover ℓa ℓb @ s; E
+      {{ _, True }}
+      {{ <PC> H0, crash_condition ℓa ℓb }}.
+  Proof.
+    iNamed 1.
+    rewrite /recover.
+    iDestruct (mapsto_na_last with "aPts") as %[sA saEq].
+    iDestruct (mapsto_na_last with "bPts") as %[sB sbEq].
+
+    (* Load [ℓa]. *)
+    wpc_bind (!_NA _)%E.
+    iApply wpc_atomic_no_mask.
+    iSplit; first iApply (prove_crash_condition with "aPer bPer aPts bPts").
+
+    iApply (wp_load_na _ _ _ _ (λ v, ⌜v = #sA⌝)%I with "[$aPts]"); first done.
+    { iModIntro. naive_solver. }
+    iIntros "!>" (?) "[aPts ->]".
+    iSplit.
+    { iModIntro. iApply (prove_crash_condition with "aPer bPer aPts bPts"). }
+
+    iModIntro.
+    wpc_pures.
+    { iApply (prove_crash_condition with "aPer bPer aPts bPts"). }
+
+    (* Load [ℓb]. *)
+    wpc_bind (!_NA _)%E.
+    iApply wpc_atomic_no_mask.
+    iSplit; first iApply (prove_crash_condition with "aPer bPer aPts bPts").
+    iApply (wp_load_na _ _ _ _ (λ v, ∃ sB', ⌜ sB ⊑ sB' ⌝ ∗ ⌜v = #sB⌝ ∗ flush_lb ℓa _ sB')%I
+              with "[$bPts]"); first done.
+    { iModIntro. iIntros (?) "(-> & (%sB' & % & #?))".
+      iSplit. { iExists _. iFrame "#". naive_solver. }
+      rewrite /ϕb. iFrame "#". naive_solver. }
+    iIntros "!>" (?) "(bPts & (%sB' & %incl2 & -> & lub))".
+    iSplit.
+    { iModIntro. iApply (prove_crash_condition with "aPer bPer aPts bPts"). }
+
+    iModIntro.
+    wpc_pures; first iApply (prove_crash_condition with "aPer bPer aPts bPts").
+
+    iDestruct (mapsto_na_flush_lb_incl with "lub aPts") as %incl; first done.
+    rewrite bool_decide_eq_false_2.
+    2: { rewrite subseteq_nat_le in incl. rewrite subseteq_nat_le in incl2. lia. }
+
+    wpc_pures; first iApply (prove_crash_condition with "aPer bPer aPts bPts").
+
+    by iModIntro.
+  Qed.
+
+  (* FIXME: Hoare triples don't work as Perennial's Hoare triples are tied to iProp. *)
+  (* Lemma wpc_incr' (ℓa ℓb : loc) : *)
+  (*   {{{ (True : dProp Σ) }}} *)
+  (*     incr_both ℓa ℓb @ 10; ⊤ *)
+  (*   {{{ RET #(); (True : dProp Σ) }}}. *)
+
+  (* Lemma wpc_incr (ℓa ℓb : loc) : *)
+  (*   {{{ (True : dProp Σ) }}} *)
+  (*     incr_both ℓa ℓb @ 10; ⊤ *)
+  (*   {{{ RET #(); (True : dProp Σ) }}} *)
+  (*   {{{ (True : dProp Σ) }}}. *)
+
+  Lemma incr_safe s E ℓa ℓb :
+    ⊢ persist_lb ℓa ϕa 0 -∗
+      persist_lb ℓb (ϕb ℓa) 0 -∗
+      ℓa ↦_{ϕa} [0] -∗
+      ℓb ↦_{ϕb ℓa} [0] -∗
+      wpr s E (incr_both ℓa ℓb) (recover ℓa ℓb)
+        (λ _, ℓa ↦_{ϕa} [0; 1] ∗ ℓb ↦_{ϕb ℓa} [0; 1]) (λ _ _, True%I).
+  Proof.
+    iIntros "a b c d".
+    iApply (idempotence_wpr _ _ _ _ _ _ (λ _, <PC> _, crash_condition ℓa ℓb)%I
+              with "[a b c d] []").
+    { iApply (wp_incr_both _ _ s E with "a b c d"). }
+    do 2 iModIntro.
+    iIntros (hG') "R".
+    iCrash.
+    iApply (wpc_recover with "R").
+  Qed.
+
+End specification.
